plumbing through stack slots in the wrapper

vale/code/arch/x64/interop/new/Vale.AsLowStar.ValeSig.fst
@@ -18,23 +18,23 @@ assume //TODO: this equivalence should be provided by Vale.Decls
 val code_equiv : squash (V.va_code == TS.tainted_code)
 
 [@__reduce__]
-let vale_pre_tl (dom:list td) =
-    n_arrow dom (V.va_state -> IX64.stack_buffer -> prop)
+let vale_pre_tl (num_b8_slots:IX64.max_slots) (dom:list td) =
+    n_arrow dom (V.va_state -> IX64.stack_buffer num_b8_slots -> prop)
 
 [@__reduce__]
-let vale_pre (dom:list td) =
+let vale_pre n (dom:list td) =
     code:V.va_code ->
-    vale_pre_tl dom
+    vale_pre_tl n dom
 
 [@__reduce__]
-let vale_post_tl (dom:list td) =
+let vale_post_tl n (dom:list td) =
     n_arrow dom
-            (s0:V.va_state -> sb:IX64.stack_buffer -> s1:V.va_state -> f:V.va_fuel -> prop)
+            (s0:V.va_state -> sb:IX64.stack_buffer n -> s1:V.va_state -> f:V.va_fuel -> prop)
 
 [@__reduce__]
-let vale_post (dom:list td) =
+let vale_post n (dom:list td) =
     code:V.va_code ->
-    vale_post_tl dom
+    vale_post_tl n dom
 
 let vale_save_reg (r:MS.reg) (s0 s1:V.va_state) =
   VS.eval_reg r s0 == VS.eval_reg r s1
@@ -91,15 +91,16 @@ let readable_one (s:ME.mem) (arg:arg) : prop =
 
 [@__reduce__]
 let readable (args:list arg) (s:ME.mem) : prop =
-  BigOps.big_and' (readable_one s) args
+    BigOps.big_and' (readable_one s) args
 
 [@__reduce__] unfold
-let vale_sig_nil (args:list arg)
+let vale_sig_nil #n
+                 (args:list arg)
                  (code:V.va_code)
-                 (pre:vale_pre_tl [])
-                 (post:vale_post_tl []) =
+                 (pre:vale_pre_tl n [])
+                 (post:vale_post_tl n []) =
     va_s0:V.va_state ->
-    stack_b:IX64.stack_buffer ->
+    stack_b:IX64.stack_buffer n ->
     Ghost (V.va_state & V.va_fuel)
      (requires
        elim_nil pre va_s0 stack_b)
@@ -113,11 +114,12 @@ let vale_sig_nil (args:list arg)
        ME.modifies (mloc_modified_args (arg_of_lb stack_b :: args)) va_s0.VS.mem va_s1.VS.mem))
 
 [@__reduce__]
-let rec vale_sig_tl (#dom:list td)
+let rec vale_sig_tl #n
+                    (#dom:list td)
                     (args:list arg)
                     (code:V.va_code)
-                    (pre:vale_pre_tl dom)
-                    (post:vale_post_tl dom)
+                    (pre:vale_pre_tl n dom)
+                    (post:vale_post_tl n dom)
   : Type =
     match dom with
     | [] ->
@@ -125,34 +127,34 @@ let rec vale_sig_tl (#dom:list td)
 
     | hd::tl ->
       x:td_as_type hd ->
-      vale_sig_tl #tl ((|hd,x|)::args) code (elim_1 pre x) (elim_1 post x)
+      vale_sig_tl #n #tl ((|hd,x|)::args) code (elim_1 pre x) (elim_1 post x)
 
 
 [@__reduce__]
-let elim_vale_sig_nil #code
+let elim_vale_sig_nil #n #code
                        (#args:list arg)
-                       (#pre:vale_pre_tl [])
-                       (#post:vale_post_tl [])
-                       (v:vale_sig_tl #[] args code pre post)
+                       (#pre:vale_pre_tl n [])
+                       (#post:vale_post_tl n [])
+                       (v:vale_sig_tl #n #[] args code pre post)
     : vale_sig_nil args code pre post
     = v
 
 [@__reduce__]
-let elim_vale_sig_cons #code
+let elim_vale_sig_cons #n #code
                        (hd:td)
                        (tl:list td)
                        (args:list arg)
-                       (pre:vale_pre_tl (hd::tl))
-                       (post:vale_post_tl (hd::tl))
+                       (pre:vale_pre_tl n (hd::tl))
+                       (post:vale_post_tl n (hd::tl))
                        (v:vale_sig_tl args code pre post)
     : x:td_as_type hd
     -> vale_sig_tl ((|hd, x|)::args) code (elim_1 pre x) (elim_1 post x)
     = v
 
 [@__reduce__]
-let vale_sig (#dom:list td)
-             (pre:vale_pre dom)
-             (post:vale_post dom)
+let vale_sig #n (#dom:list td)
+             (pre:vale_pre n dom)
+             (post:vale_post n dom)
   : Type =
     code:V.va_code ->
     win:bool ->
