vale/code/arch/x64/interop/new/Vale.AsLowStar.MemoryHelpers.fsti
@@ -53,29 +53,32 @@ val readable_live (#t:_) (x:lowstar_buffer t) (s:ME.mem)
         B.live (Interop.Adapters.hs_of_mem s) x)
 
 val buffer_readable_reveal 
+  (#n:_)
   (bt:ME.base_typ)
   (x:lowstar_buffer (ME.TBase bt)) 
   (args:IX64.arity_ok arg)
   (h0:HS.mem)
-  (stack:IX64.stack_buffer{mem_roots_p h0 (arg_of_lb stack::args)}) : Lemma (
+  (stack:IX64.stack_buffer n{mem_roots_p h0 (arg_of_lb stack::args)}) : Lemma (
     let mem = Interop.Adapters.mk_mem (arg_of_lb stack::args) h0 in
     ME.buffer_readable mem (as_vale_buffer #(ME.TBase bt) x) <==>
       List.memP x (Interop.Adapters.ptrs_of_mem mem))
 
 val get_heap_mk_mem_reveal
+  (#n:_)
   (args:IX64.arity_ok arg)
   (h0:HS.mem)
-  (stack:IX64.stack_buffer{mem_roots_p h0 (arg_of_lb stack::args)}) : Lemma
+  (stack:IX64.stack_buffer n{mem_roots_p h0 (arg_of_lb stack::args)}) : Lemma
   (let mem = Interop.Adapters.mk_mem (arg_of_lb stack::args) h0 in
    Interop.Adapters.liveness_disjointness (arg_of_lb stack::args) h0;
    MES.get_heap mem == IM.down_mem h0 IA.addrs (Interop.Adapters.args_b8 (arg_of_lb stack::args)))
 
 val buffer_as_seq_reveal
+  (#n:_)
   (t:ME.base_typ)
   (x:lowstar_buffer (ME.TBase t))
   (args:IX64.arity_ok arg)
   (h0:HS.mem)
-  (stack:IX64.stack_buffer{mem_roots_p h0 (arg_of_lb stack::args)}) : Lemma
+  (stack:IX64.stack_buffer n{mem_roots_p h0 (arg_of_lb stack::args)}) : Lemma
   (let y = as_vale_buffer x in
   let mem = Interop.Adapters.mk_mem (arg_of_lb stack::args) h0 in
   assume (t <> ME.TUInt128); // TODO: UInt128
