vale/specs/interop/Interop.X64.fst
@@ -9,7 +9,7 @@ module TS = X64.Taint_Semantics_s
 module IA = Interop.Assumptions
 module ST = FStar.HyperStack.ST
 
-let wrap_variadic c args #pre_rel #post_rel predict =
+let wrap_variadic c num_b8_slots args #pre_rel #post_rel predict =
   let h0 = ST.get () in
   let h0' = h0 in
   assert (mem_roots_p h0' args);
@@ -17,7 +17,7 @@ let wrap_variadic c args #pre_rel #post_rel predict =
   let push_h0 = ST.get () in
   B.fresh_frame_modifies h0' push_h0;
   mem_roots_p_modifies_none args h0' push_h0;
-  let stack_b : stack_buffer = B.alloca (UInt8.uint_to_t 0) (UInt32.uint_to_t 24) in
+  let stack_b : stack_buffer num_b8_slots = B.alloca (UInt8.uint_to_t 0) (UInt32.uint_to_t num_b8_slots) in
   let alloc_push_h0 = ST.get () in
   assert (HS.fresh_frame h0 push_h0);
   mem_roots_p_modifies_none args push_h0 alloc_push_h0;
@@ -32,7 +32,7 @@ let wrap_variadic c args #pre_rel #post_rel predict =
       (fun h0' -> h0' == alloc_push_h0)
       (fun h0' ->
         let va_s0, mem_s0 =
-          create_initial_trusted_state args h0' stack_b in
+          create_initial_trusted_state num_b8_slots args h0' stack_b in
         let (fuel, final_mem) = predict h0 va_s0 push_h0 alloc_push_h0 stack_b in
         assert (B.frameOf stack_b = HS.get_tip h0');
         assert (B.live h0' stack_b);
@@ -42,16 +42,17 @@ let wrap_variadic c args #pre_rel #post_rel predict =
       ) in
   ST.pop_frame ();
   assert (ST.equal_domains alloc_push_h0 (Adapters.hs_of_mem final_mem));
-  Ghost.hide (As_lowstar_sig_ret args push_h0 alloc_push_h0 stack_b fuel final_mem)
+  Ghost.hide (As_lowstar_sig_ret num_b8_slots args push_h0 alloc_push_h0 stack_b fuel final_mem)
 
 let rec wrap_aux
     (c:TS.tainted_code)
+    (num_b8_slots:max_slots)
     (dom:list td)
     (args:list arg{arity_ok_2 dom args})
     (pre_rel:rel_gen_t c dom args (prediction_pre_rel_t c))
-    (post_rel:rel_gen_t c dom args (prediction_post_rel_t c))
-    (predict:prediction_t c dom args pre_rel post_rel)
-  : as_lowstar_sig_t c dom args pre_rel post_rel predict
+    (post_rel:rel_gen_t c dom args (prediction_post_rel_t c num_b8_slots))
+    (predict:prediction_t c num_b8_slots dom args pre_rel post_rel)
+  : as_lowstar_sig_t c num_b8_slots dom args pre_rel post_rel predict
   = match dom with
     | [] ->
       let f () :
@@ -59,29 +60,31 @@ let rec wrap_aux
            (requires fun h0 ->
              mem_roots_p h0 args /\ elim_rel_gen_t_nil pre_rel h0)
            (ensures fun h0 ret h1 ->
-             as_lowstar_sig_post c args h0 #pre_rel #post_rel (elim_predict_t_nil predict) ret h1) =
-        wrap_variadic c args (elim_predict_t_nil predict)
+             as_lowstar_sig_post c num_b8_slots args h0 #pre_rel #post_rel (elim_predict_t_nil predict) ret h1) =
+        wrap_variadic c num_b8_slots args (elim_predict_t_nil predict)
       in
-      f <: as_lowstar_sig_t c [] args pre_rel post_rel predict
+      f <: as_lowstar_sig_t c num_b8_slots [] args pre_rel post_rel predict
 
     | hd::tl ->
       fun (x:td_as_type hd) ->
-      wrap_aux c tl
+      wrap_aux c num_b8_slots tl
         (x ++ args)
         (elim_rel_gen_t_cons hd tl pre_rel x)
         (elim_rel_gen_t_cons hd tl post_rel x)
         (elim_predict_t_cons hd tl predict x)
 
-let wrap c dom #pre_rel #post_rel predict = wrap_aux c dom [] pre_rel post_rel predict
+let wrap c num_b8_slots dom #pre_rel #post_rel predict =
+  wrap_aux c num_b8_slots dom [] pre_rel post_rel predict
 
 let rec wrap_aux_weak
     (c:TS.tainted_code)
+    (num_b8_slots:max_slots)
     (dom:list td)
     (args:list arg{arity_ok_2 dom args})
     (pre_rel:rel_gen_t c dom args (prediction_pre_rel_t c))
-    (post_rel:rel_gen_t c dom args (prediction_post_rel_t c))
-    (predict:prediction_t c dom args pre_rel post_rel)
-  : as_lowstar_sig_t_weak c dom args pre_rel post_rel predict
+    (post_rel:rel_gen_t c dom args (prediction_post_rel_t c num_b8_slots))
+    (predict:prediction_t c num_b8_slots dom args pre_rel post_rel)
+  : as_lowstar_sig_t_weak c num_b8_slots dom args pre_rel post_rel predict
   = match dom with
     | [] ->
       let f () :
@@ -89,17 +92,18 @@ let rec wrap_aux_weak
            (requires fun h0 ->
              mem_roots_p h0 args /\ elim_rel_gen_t_nil pre_rel h0)
            (ensures fun h0 ret h1 ->
-             as_lowstar_sig_post_weak c args h0 #pre_rel #post_rel (elim_predict_t_nil predict) ret h1) =
-         wrap_variadic c args (elim_predict_t_nil predict)
+             as_lowstar_sig_post_weak c num_b8_slots args h0 #pre_rel #post_rel (elim_predict_t_nil predict) ret h1) =
+         wrap_variadic c num_b8_slots args (elim_predict_t_nil predict)
       in
-      f <: as_lowstar_sig_t_weak c [] args pre_rel post_rel predict
+      f <: as_lowstar_sig_t_weak c num_b8_slots [] args pre_rel post_rel predict
 
     | hd::tl ->
       fun (x:td_as_type hd) ->
-      wrap_aux_weak c tl
+      wrap_aux_weak c num_b8_slots tl
         (x ++ args)
         (elim_rel_gen_t_cons hd tl pre_rel x)
         (elim_rel_gen_t_cons hd tl post_rel x)
         (elim_predict_t_cons hd tl predict x)
 
-let wrap_weak c dom #pre_rel #post_rel predict = wrap_aux_weak c dom [] pre_rel post_rel predict
+let wrap_weak c num_b8_slots dom #pre_rel #post_rel predict =
+  wrap_aux_weak c num_b8_slots dom [] pre_rel post_rel predict
